Validate submission 59a153c6-28ee-4349-97d5-c09cf4414296
Co-authored-by: fkiene <46886660+fkiene@users.noreply.github.com>

Challenge/Modexp/Submission/Proofs/Bytecode/Artifact.lean
@@ -2360,9 +2360,24 @@ def submissionInstructions : List Instr :=
  YulEvmCompiler.Instr.push 1 32,
  YulEvmCompiler.Instr.push 0 0,
  YulEvmCompiler.Instr.op EvmSemantics.Operation.RETURN,
+YulEvmCompiler.Instr.op EvmSemantics.Operation.JUMPDEST,
+YulEvmCompiler.Instr.op (EvmSemantics.Operation.Dup { idx := 1 }),
+YulEvmCompiler.Instr.op EvmSemantics.Operation.ISZERO,
+YulEvmCompiler.Instr.push 2 3593,
+YulEvmCompiler.Instr.op EvmSemantics.Operation.JUMPI,
+YulEvmCompiler.Instr.push 2 9344,
+YulEvmCompiler.Instr.op EvmSemantics.Operation.MLOAD,
+YulEvmCompiler.Instr.push 2 2048,
+YulEvmCompiler.Instr.push 2 1024,
+YulEvmCompiler.Instr.op EvmSemantics.Operation.MCOPY,
+YulEvmCompiler.Instr.push 2 1832,
+YulEvmCompiler.Instr.op EvmSemantics.Operation.JUMP,
+YulEvmCompiler.Instr.op EvmSemantics.Operation.JUMPDEST,
+YulEvmCompiler.Instr.push 2 1789,
+YulEvmCompiler.Instr.op EvmSemantics.Operation.JUMP
 ]
 
-theorem submissionInstructions_count : submissionInstructions.length = 2338 := by
+theorem submissionInstructions_count : submissionInstructions.length = 2353 := by
   decide
 
 theorem assemble_submissionInstructions :
